theories/lifetime/frac_borrow.v
@@ -11,7 +11,7 @@ Definition frac_bor `{invG Σ, lftG Σ, frac_borG Σ} κ (Φ : Qp → iProp Σ) 
   (∃ γ κ', κ ⊑ κ' ∗ &shr{κ'} ∃ q, Φ q ∗ own γ q ∗
                        (⌜q = 1%Qp⌝ ∨ ∃ q', ⌜(q + q' = 1)%Qp⌝ ∗ q'.[κ']))%I.
 Notation "&frac{ κ } P" := (frac_bor κ P)
-  (format "&frac{ κ } P", at level 20, right associativity) : uPred_scope.
+  (format "&frac{ κ }  P", at level 20, right associativity) : uPred_scope.
 
 Section frac_bor.
   Context `{invG Σ, lftG Σ, frac_borG Σ}.
