theories/typing/tests/init_prod.v
@@ -12,7 +12,7 @@ Section rebor.
        let: "x'" := !"x" in let: "y'" := !"y" in
        let: "r" := new [ #2] in
        "r" +ₗ #0 <- "x'";; "r" +ₗ #1 <- "y'";;
-       delete [ #1; "x"] ;; delete [ #1; "y"] ;; "return" ["r":expr].
+       delete [ #1; "x"] ;; delete [ #1; "y"] ;; "return" ["r"].
 
   Lemma init_prod_type :
     typed_instruction_ty [] [] [] init_prod
