theories/typing/tests/unbox.v
@@ -11,7 +11,7 @@ Section unbox.
     funrec: <> ["b"] :=
        let: "b'" := !"b" in let: "bx" := !"b'" in
        letalloc: "r" := "bx" +ₗ #0 in
-       delete [ #1; "b"] ;; "return" ["r":expr].
+       delete [ #1; "b"] ;; "return" ["r"].
 
   Lemma ubox_type :
     typed_instruction_ty [] [] [] unbox
@@ -20,7 +20,7 @@ Section unbox.
   Proof.
     apply type_fn; try apply _. move=> /= α ret b. inv_vec b=>b. simpl_subst.
     eapply type_deref; try solve_typing. by apply read_own_move. done.
-      intros b'; simpl_subst.
+    intros b'; simpl_subst.
     eapply type_deref_uniq_own; (try solve_typing)=>bx; simpl_subst.
     eapply type_letalloc_1; (try solve_typing)=>r. simpl_subst.
     eapply type_delete; try solve_typing.
